Merge com o file do Edu

Queue.dfy
@@ -1,32 +1,46 @@
 class {:autocontracts} Queue {
-      // Atributos
+
+  // Atributos
   var circularQueue: array<int>;
-  var rear: int;
-  var front: int;
+  var rear: nat;  // cauda
+  var front: nat; // head
+  var queueSize: nat;
+  var counter: nat;
 
   // Abstração
   ghost var Content: seq<int>;
 
   // Predicado
   ghost predicate Valid()
-    {
-    
-    }
+  {
+    0 <= counter <= circularQueue.Length &&
+    0 <= front &&
+    0 <= rear &&
+    queueSize == circularQueue.Length &&
+    Content == circularQueue[0..circularQueue.Length]
+  }
 
-    // Construtor
-    constructor()
-      ensures Content == []
-    {
+  // Construtor
+  constructor()
+    ensures circularQueue.Length == 0
+    ensures front == 0 && rear == 0
+    ensures Content == [] // REVISAR
+    ensures counter == 0
+  {
     circularQueue := new int[0];
     rear := 0;
     front := 0;
+    queueSize := 0;
     Content := [];
-    }
+    counter := 0;
+  }
 
   // Métodos
 
+  // 1 - 
   method insert(item: int)
-    ensures Content == old(Content) + [item]
+    // ensures Content == old(Content) + [item];
+    
 
   method remove(item: int)
     requires |Content| > 0
@@ -34,13 +48,53 @@ class {:autocontracts} Queue {
     ensures Content == old(Content)[1..]
 
   method size() returns (size:nat)
-    ensures size == |Content|
+    ensures size == counter
+  {
+    size := counter;
+  }
+
+  method isEmpty() returns (isEmpty: bool)
+    ensures isEmpty == (counter == 0);
+  {
+    isEmpty := if counter == 0 then true else false;
+  }
+
+  method contains(item: int) returns (contains: bool)
+    ensures contains == true ==> item in circularQueue[..]
+    ensures contains == false ==> item !in circularQueue[..]
     ensures Content == old(Content)
-  
-  method isEmpty() returns (isEmpty:bool)
-    ensures isEmpty == (|Content| == 0)
+  {
+    var i: nat := 0;
+    contains := false;
+
+    while (i < circularQueue.Length)
+      decreases circularQueue.Length - i
+      invariant 0 <= i <= circularQueue.Length
+      invariant !contains ==> forall j :: 0 <= j < i ==> circularQueue[j] != item
+    {
+      if (circularQueue[i] == item) {
+        contains := true;
+        break;
+      }
+      i := i + 1;
+    }
+  }
 
   // TODO
-  // method contains()
   // method mergeQueues() returns (mergedQueue:array<int>)
+}
+
+method Main ()
+{
+  var circularQueue := new Queue();
+  assert circularQueue.circularQueue.Length == 0;
+  assert circularQueue.Content == [];
+  assert circularQueue.Content != [1];
+
+  var isQueueEmpty := circularQueue.isEmpty();
+  assert isQueueEmpty == true;
+
+  var queueSize := circularQueue.size();
+  assert queueSize == 0;
+
 }
